Source/DafnyStandardLibraries/src/Std/Parsers/String/StringParsers.dfy
@@ -1,7 +1,39 @@
+module Std.Parsers.InputString refines AbstractInput {
+  datatype Input_ = Input(data: seq<char>, start: int, end: int) {
+    ghost predicate Valid() {
+      0 <= start <= end <= |data|
+    }
+    function ToString(): string {
+      data[start..end]
+    }
+  }
+
+  type Input = x: Input_ | x.Valid()
+  type C = char
+
+  function View(self: Input): (r: seq<C>)
+    ensures |View(self)| == Length(self) {
+    self.data[self.start..self.end]
+  }
+  function Length(self: Input): nat { self.end - self.start  }
+  function CharAt(self: Input, i: int): C
+    ensures CharAt(self, i) == View(self)[i]  { self.data[self.start + i] }
+  function Drop(self: Input, start: int): Input
+    ensures View(self)[start..] == View(Drop(self, start)) { Input(self.data, self.start + start, self.end) }
+  function Slice(self: Input, start: int, end: int): Input
+    ensures View(self)[start..end] == View(Slice(self, start, end)) { Input(self.data, self.start + start, self.start + end) }
+  predicate Equals(self: Input, other: Input)
+    ensures Equals(self, other) <==> View(self) == View(other)
+  {
+    self == other
+  }
+}
+
 module Std.Parsers.StringParsers refines Core {
   export StringParsers reveals *
   export Export extends Core
     provides
+      CodeLocation,
       Char,
       Digit,
       DigitNumber,
@@ -14,7 +46,7 @@ module Std.Parsers.StringParsers refines Core {
       WS
     reveals C
 
-  type C = char
+  import A = InputString
 
   // ##################################
   // String-specific parser combinators
@@ -47,7 +79,7 @@ module Std.Parsers.StringParsers refines Core {
     // A parser that returns the current char as a number if it is one
   {
     Map(Digit(), (c: char) =>
-          var d := digitToInt(c);
+          var d := DigitToInt(c);
           var n: nat := if d >= 0 then d else 0;
           n
     )
@@ -78,8 +110,9 @@ module Std.Parsers.StringParsers refines Core {
     // A parser that succeeds only if the input starts with the given string
     // Its failure is recoverable, so it's possible to branch to something else
   {
-    (input: string) =>
-      if |expected| <= |input| && input[0..|expected|] == expected then Success(expected, input[|expected|..])
+    (input: Input) =>
+      if |expected| <= A.Length(input) && A.Slice(input, 0, |expected|).ToString() == expected then
+        Success(expected, A.Drop(input, |expected|))
       else Failure(Recoverable, FailureData("expected '"+expected+"'", input, Option.None))
   }
 
@@ -95,17 +128,68 @@ module Std.Parsers.StringParsers refines Core {
     else str + repeat_(str, n-1)
   }
 
-  method ExtractLineCol(input: string, pos: nat)
-    returns (lineNumber: nat, lineStr: string, colNumber: nat)
-    // Returns the line number, the extracted line, and the column number
-    // corresponding to a given position in the given input
+  datatype CodeLocation = CodeLocation(lineNumber: nat, colNumber: nat, lineStr: string)
+  datatype ExtractLineMutableState = ExtractLineMutableState(input: string, pos: nat, startLinePos: nat, i: nat, lineNumber: nat, colNumber: nat)
+
+  ghost function ExtractLineColSpecAux(vars: ExtractLineMutableState): (res: ExtractLineMutableState)
+    requires 0 <= vars.startLinePos <= vars.i <= |vars.input|
+    decreases |vars.input| - vars.i
+    ensures 0 <= res.startLinePos <= res.i <= |res.input|
+    ensures !(res.i < |res.input| && res.i != res.pos) // Negation of the while guard
   {
+    if vars.i < |vars.input| && vars.i != vars.pos then
+      var colNumber := vars.colNumber + 1;
+      if vars.input[vars.i] == '\r' && vars.i + 1 < |vars.input| && vars.input[vars.i+1] == '\n' then
+        //var startLinePos := i + 1; // ORIGINAL BUG: vars.i + 1
+        ExtractLineColSpecAux(ExtractLineMutableState(vars.input, vars.pos, vars.i + 2, vars.i + 2, vars.lineNumber + 1, 0))
+      else if vars.input[vars.i] in "\r\n" then
+        var lineNumber := vars.lineNumber + 1;
+        var colNumber := 0;
+        var startLinePos := vars.i + 1;
+        ExtractLineColSpecAux(ExtractLineMutableState(vars.input, vars.pos, startLinePos, vars.i + 1, lineNumber, colNumber))
+      else
+        ExtractLineColSpecAux(ExtractLineMutableState(vars.input, vars.pos, vars.startLinePos, vars.i + 1, vars.lineNumber, colNumber))
+    else
+      vars
+  }
+  opaque ghost function ExtractLineColSpecAux2(vars: ExtractLineMutableState): (res: ExtractLineMutableState)
+    requires 0 <= vars.startLinePos <= vars.i <= |vars.input|
+    ensures 0 <= res.startLinePos <= res.i <= |res.input|
+    decreases |vars.input| - vars.i
+    ensures !(res.i < |res.input| && res.input[res.i] !in "\r\n") // Negation of the while guard  
+  {
+     if vars.i < |vars.input| && vars.input[vars.i] !in "\r\n" then // Second loop
+      ExtractLineColSpecAux2(vars.(i := vars.i + 1))
+    else
+      vars
+  }
+  opaque ghost function ToCodeLocation(vars: ExtractLineMutableState): CodeLocation
+    requires 0 <= vars.startLinePos <= vars.i <= |vars.input|
+  {
+    CodeLocation(vars.lineNumber, vars.colNumber, vars.input[vars.startLinePos..vars.i])
+  }
+  // Returns the line number, the extracted line, and the column number
+  // corresponding to a given position in the given input
+  // If you ask, the method was created first and then lifted up to a function
+  opaque function ExtractLineCol(input: string, pos: nat):  (output: CodeLocation)
+  {
+    var vars := ExtractLineColSpecAux(ExtractLineMutableState(input, pos, 0, 0, 1, 0));
+    var vars := ExtractLineColSpecAux2(vars);
+    ToCodeLocation(vars)
+  } by method {
+    var lineNumber, colNumber, lineStr;
     lineNumber := 1;
     var startLinePos: nat := 0;
     colNumber := 0;
     var i := 0;
+    reveal ExtractLineCol();
+    assert ExtractLineCol(input, pos) == ToCodeLocation(ExtractLineColSpecAux2(ExtractLineColSpecAux(ExtractLineMutableState(input, pos, startLinePos, i, lineNumber, colNumber))));
     while i < |input| && i != pos
       invariant 0 <= startLinePos <= i <= |input|
+      invariant 
+        ToCodeLocation(ExtractLineColSpecAux2(ExtractLineColSpecAux(
+          ExtractLineMutableState(input, pos, startLinePos, i, lineNumber, colNumber))))
+        == ExtractLineCol(input, pos)
     {
       colNumber := colNumber + 1;
       if input[i] == '\r' && i + 1 < |input| && input[i+1] == '\n' {
@@ -120,21 +204,30 @@ module Std.Parsers.StringParsers refines Core {
       }
       i := i + 1;
     }
+    assert ExtractLineCol(input, pos) == ToCodeLocation(ExtractLineColSpecAux2(ExtractLineMutableState(input, pos, startLinePos, i, lineNumber, colNumber)));
+    reveal ExtractLineColSpecAux2();
     while i < |input| && input[i] !in "\r\n"
-      invariant startLinePos <= i <= |input|
+      invariant 0 <= startLinePos <= i <= |input|
+      invariant 
+        ToCodeLocation(ExtractLineColSpecAux2(
+          ExtractLineMutableState(input, pos, startLinePos, i, lineNumber, colNumber)))
+        == ExtractLineCol(input, pos)
     {
+      assert 
+        ToCodeLocation(ExtractLineColSpecAux2(
+          ExtractLineMutableState(input, pos, startLinePos, i + 1, lineNumber, colNumber)))
+        == ExtractLineCol(input, pos);
       i := i + 1;
     }
+    assert ExtractLineCol(input, pos) == ToCodeLocation(ExtractLineMutableState(input, pos, startLinePos, i, lineNumber, colNumber));
     lineStr := input[startLinePos..i];
-  }
-
-  function NatToString(input: nat): string {
-    if input < 10 then "0123456789"[input..input + 1] else
-    NatToString(input / 10) + NatToString(input % 10)
+    output := CodeLocation(lineNumber, colNumber, lineStr);
+    reveal ToCodeLocation();
+    assert ExtractLineCol(input, pos) == output;
   }
 
   function DebugSummary(input: string): string {
-    NatToString(|input|) + " \"" +
+    IntToString(|input|) + " \"" +
     (if |input| > 0 then
       match input[0] {
         case '\n' => "\\n"
@@ -162,47 +255,47 @@ module Std.Parsers.StringParsers refines Core {
   method {:print} PrintDebugSummaryOutput<R>(name: string, input: string, result: ParseResult<R>) {
     print "< ", DebugNameSummary(name, input);
     if result.Failure? {
-      var failureMessage := FailureToString(input, result);
-      print "| R: ", DebugSummary(result.Remaining());
-      if |result.Remaining()| < |input| {
+      print "| R: ", DebugSummary(A.View(result.Remaining()));
+      if A.Length(result.Remaining()) < |input| {
         print "| Was committed\n";
       }
-      print "| " + NewIndent(failureMessage, "| "), "\n";
+      print "| " + NewIndent(FailureToString(input, result), "| "), "\n";
     } else {
       print " (Success)\n";
     }
   }
 
-  method FailureToString<R>(input: string, result: ParseResult<R>, printPos: int := -1) returns (failure: string)
+  opaque function FailureToString<R>(input: string, result: ParseResult<R>, printPos: int := -1): (failure: string)
     // Util to print the line, the column, and all the error messages
     // associated to a given parse failure
     requires result.Failure?
     decreases result.data
   {
-    failure := "";
-    failure := failure +
-    if printPos == -1 then
-      (if result.level == Fatal then "Fatal error" else "Error") + ":\n"
-    else "";
-    var pos: int := |input| - |result.data.remaining|; // Need the parser to be Valid()
-    pos := if pos < 0 then // Could be proved false if parser is Valid()
-      0
-    else
-      pos;
-    if printPos != pos {
-      var line, lineStr, col := ExtractLineCol(input, pos);
-      failure := failure + NatToString(line) + ": " + lineStr + "\n" +
-      repeat_(" ", col + 2 + |intToString(line)|) + "^" + "\n";
-    }
-    failure := failure + result.data.message;
-    if result.data.next.Some? {
-      failure := failure + ", or\n";
+    var failure := "";
+    var failure := failure +
+      if printPos == -1 then
+        (if result.level == Fatal then "Fatal error" else "Error") + ":\n"
+      else "";
+    var pos: int := |input| - A.Length(result.data.remaining); // Need the parser to be Valid()
+    var pos :=
+      if pos < 0 then // Could be proved false if parser is Valid()
+        0
+      else
+        pos;
+    var failure :=
+    if printPos == pos then failure else
+      var output := ExtractLineCol(input, pos);
+      var CodeLocation(line, col, lineStr) := output;
+      failure + IntToString(line) + ": " + lineStr + "\n" +
+      repeat_(" ", col + 2 + |IntToString(line)|) + "^" + "\n";
+    var failure := failure + result.data.message;
+    if result.data.next.Some? then
+      var failure := failure + ", or\n";
       var subFailure := FailureToString<R>(input, Failure(result.level, result.data.next.value), pos);
-      failure := failure + subFailure;
-      return failure;
-    } else {
-      failure := failure + "\n";
-      return failure;
-    }
+      var failure := failure + subFailure;
+      failure
+    else
+      var failure := failure + "\n";
+      failure
   }
 }
